<?xml version="1.0" encoding="UTF-8"?>

<section xml:id="sec-dualitytheory" xmlns:xi="http://www.w3.org/2001/XInclude">
  <title>Duality Theory</title>
  <introduction>
    <p> In this section, we establish the theoretical underpinnings of duality. This is a proof heavy section.</p>
  </introduction>   
  

  <observation>
    <statement>
      <p>
        Recall the primal maximization problem <xref ref="activity-maxslack"/>, and the corresponding
        dual minimization problem <xref ref="definition-dual"/>. By letting 
        <me>A = \begin{bmatrix} a_{11} \amp a_{12} \amp \cdots \amp a_{1m} \\ 
          a_{21} \amp a_{22} \amp \cdots \amp a_{2m} \\
          \vdots \amp \vdots \amp \ddots \amp \vdots \\
          a_{n1} \amp a_{n2} \amp \cdots \amp a_{nm} \end{bmatrix}, 
        b = \begin{bmatrix} b_1 \\ b_2 \\ \vdots \\ b_n \end{bmatrix}, 
      c^{\top}= \begin{bmatrix}c_1 \amp c_2\amp \cdots \amp c_m \end{bmatrix}, d=d</me>
  
      

      </p>
      <p>
        We can rephrase the primal max problem as follows: Maximize <m>f = c^{\top}\mathbf{x}-d</m> for
        <m>\mathbf{x}\in \mathbb{R}^m</m> subject to <me>A\mathbf{x}\leq b, \mathbf{x}\geq 0.</me>
        Here, we understand <m>\leq, \geq </m> to denote entrywise inequality.
      </p>

      <p>
        Likewise, we can rephrase the dual min problem as follows: Minimize <m>g = \mathbf{y}^{\top}b-d</m> for
        <m>\mathbf{y}\in \mathbb{R}^n</m> subject to <me> \mathbf{y}^{\top}A\geq c^{\top}, \mathbf{y}\geq 0.</me>
      </p>
    </statement>
  </observation>

  <activity xml:id="activity-weakduality">
    <introduction>
      <statement>
        <p>
          In this activity, we explore a foundational relationship between the primal max 
          problem and it's dual, called <em>weak duality</em>.
        </p>
      </statement>
    </introduction>
    <task>
      <statement>
        <p>
          Consider the matrix product <m>\mathbf{y}^{\top}A\mathbf{x}</m>.  Use this product to show that <m>g\geq f</m>.
        </p>
      </statement>
    </task>
    <task>
      <statement>
        <p>
          Suppose there were feasible <m>\mathbf{x_0}, \mathbf{y_0}</m> for which <m>f(\mathbf{x_0},)= g(\mathbf{y_0})</m>.  What 
          then must be true about these solutions?  Can we prove our assertion?
        </p>
      </statement>
    </task>
    <task>
      <statement>
        <p>
          Recall <xref ref="activity-insurance"/> and <xref ref="exploration-witch"/>.  Consider the primal
          max and dual min of the associated problems.  How does our assertion fit these problems?
        </p>
      </statement>
    </task>
    <task>
      <statement>
        <p>
          Come up with a primal max problem (and corresponding min dual) where <m>A, b, c, d, \mathbf{x}, \mathbf{y}</m>
          all have <em>integer</em> values, so that the primal max and dual min problems achieve optimal solutions <m>\mathbf{x_0}, \mathbf{y_0}</m>,
          where <m>f(\mathbf{x_0}) \lt g(\mathbf{y_0})</m>.
        </p>
      </statement>
      
    </task>
    <task>
      <statement>
        <p>
          Using the same values for <m>A, b, c, d</m> for the problem we just constructed, suppose we relax the condition that all our values must be integers.
          What can we say about the optimal solutions then?
        </p>
      </statement>
    </task>
  </activity>

  <p>
    What we have proven is the following:
  </p>

  <proposition xml:id="prop-weakduality">
    <idx>weak duality theorem</idx>
    <idx>theorem, weak duality</idx>
    <statement>
      <p>
        For a primal maximization problem with objective function <m>f</m> and dual objective <m>g</m>,
        we have that <me>f\leq g.</me>
      </p>
      <p>
        In particular, if there is a feasible primal solution <m>\x^*</m> and feasible dual solution <m>\y^*</m> such that
        <me>f(\x^*)=g(\y^*)</me> then <m>\x^*, \y^*</m> are optimal solutions for the primal and dual problems respectively.  
      </p>
    </statement>
  </proposition>

  <p>
    We have now that if <m>f=g</m> for a pair of feasible solutions, then we have optimality
    for both problems.  It would be good if the converse were also true.  This is encapsulated by the following
    theorem.
  </p>

  <theorem xml:id="thm-strongduality">
    <title>The Strong Duality Theorem</title>
    <idx>strong duality theorem</idx>
    <idx>theorem, strong duality</idx>
    <statement>
      <p>
        Given a pair of primal max-dual min problems, the primal max problem as an optimal solution 
        <m>\x^*</m> if and only if the dual min problem has an optimal solution <m>\y^*</m>.  Moreover,
        <m>f(\x^*)=g(\y^*)</m>.
      </p>
    </statement>
  </theorem>

  <p>
    To prove this, we recall the idea we explored in <xref ref="sec-sensitivity"/>
    that dual variables were coefficients or weights of normal variables of the bounding
    hyperplanes.
  </p>

  <activity xml:id = "activity-sampleSD">
    <introduction>
      <p>
        Before we delve into the proof, we illustrate the idea with a constrained case.  Consider a canonical optimization problem captured by the following tableau (we assume for simplicities sake to let <m>d=0</m>):
        <tabular halign="center">
          <row>
            <cell halign="left">
            </cell>
            <cell bottom="medium">
              <m>x_1</m>
            </cell>
            <cell bottom="medium">
              <m>x_2</m>
            </cell>
            <cell bottom="medium">
              <m>x_3</m>
            </cell>
            <cell bottom="medium">
              <m>x_4</m>
            </cell>
            <cell bottom="medium">
              <m>-1</m>
            </cell>
            <cell halign="left">
            </cell>
          </row>
          <row>
            <cell halign="left" right="medium">
            </cell>
            <cell>
              <m>a_{11}</m>
            </cell>
            <cell>
              <m>a_{12}</m>
            </cell>
            <cell>
              <m>a_{13}</m>
            </cell>
            <cell right="medium">
              <m>a_{14}</m>
            </cell>
            <cell right="medium">
              <m>b_1</m>
            </cell>
            <cell halign="left">
              <m>=-t_1</m>
            </cell>
          </row>

          <row>
            <cell halign="left" right="medium">
            </cell>
            <cell>
              <m>a_{21}</m>
            </cell>
            <cell>
              <m>a_{22}</m>
            </cell>
            <cell>
              <m>a_{23}</m>
            </cell>
            <cell right="medium">
              <m>a_{24}</m>
            </cell>
            <cell right="medium">
              <m>b_2</m>
            </cell>
            <cell halign="left">
              <m>=-t_2</m>
            </cell>
          </row>
          
          <row>
            <cell halign="left" right="medium">
            </cell>
            <cell bottom="medium">
              <m>a_{13}</m>
            </cell>
            <cell bottom="medium">
              <m>a_{23}</m>
            </cell>
            <cell bottom="medium">
              <m>a_{33}</m>
            </cell>
            <cell right="medium" bottom="medium">
              <m>a_{43}</m>
            </cell>
            <cell right="medium" bottom="medium">
              <m>b_3</m>
            </cell>
            <cell halign="left">
              <m>=-t_3</m>
            </cell>
          </row>
          <row>
            <cell halign="left" right="medium">
            </cell>
            <cell bottom="medium">
              <m>c_1</m>
            </cell>
            <cell bottom="medium">
              <m>c_2</m>
            </cell>
            <cell bottom="medium">
              <m>c_3</m>
            </cell>
            <cell right="medium" bottom="medium">
              <m>c_4</m>
            </cell>
            <cell right="medium" bottom="medium">
              <m>0</m>
            </cell>
            <cell halign="left">
              <m>=f</m>
            </cell>
          </row>
        </tabular>
      </p>
      <p>
        Which after pivoting achieves optimality with the following tableau:
        <tabular halign="center">
          <row>
            <cell halign="left">
            </cell>
            <cell bottom="medium">
              <m>t_3</m>
            </cell>
            <cell bottom="medium">
              <m>x_3</m>
            </cell>
            <cell bottom="medium">
              <m>x_1</m>
            </cell>
            <cell bottom="medium">
              <m>t_2</m>
            </cell>
            <cell bottom="medium">
              <m>-1</m>
            </cell>
            <cell halign="left">
            </cell>
          </row>
          <row>
            <cell halign="left" right="medium">
            </cell>
            <cell>
              <m>a_{11}^*</m>
            </cell>
            <cell>
              <m>a_{12}^*</m>
            </cell>
            <cell>
              <m>a_{13}^*</m>
            </cell>
            <cell right="medium">
              <m>a_{14}^*</m>
            </cell>
            <cell right="medium">
              <m>b_1^*</m>
            </cell>
            <cell halign="left">
              <m>=-x_4</m>
            </cell>
          </row>

          <row>
            <cell halign="left" right="medium">
            </cell>
            <cell>
              <m>a_{21}^*</m>
            </cell>
            <cell>
              <m>a_{22}^*</m>
            </cell>
            <cell>
              <m>a_{23}^*</m>
            </cell>
            <cell right="medium">
              <m>a_{24}^*</m>
            </cell>
            <cell right="medium">
              <m>b_2^*</m>
            </cell>
            <cell halign="left">
              <m>=-t_1</m>
            </cell>
          </row>
          
          <row>
            <cell halign="left" right="medium">
            </cell>
            <cell bottom="medium">
              <m>a_{13}^*</m>
            </cell>
            <cell bottom="medium">
              <m>a_{23}^*</m>
            </cell>
            <cell bottom="medium">
              <m>a_{33}^*</m>
            </cell>
            <cell right="medium" bottom="medium">
              <m>a_{43}^*</m>
            </cell>
            <cell right="medium" bottom="medium">
              <m>b_3^*</m>
            </cell>
            <cell halign="left">
              <m>=-x_2</m>
            </cell>
          </row>
          <row>
            <cell halign="left" right="medium">
            </cell>
            <cell bottom="medium">
              <m>c_1^*</m>
            </cell>
            <cell bottom="medium">
              <m>c_2^*</m>
            </cell>
            <cell bottom="medium">
              <m>c_3^*</m>
            </cell>
            <cell right="medium" bottom="medium">
              <m>c_4^*</m>
            </cell>
            <cell right="medium" bottom="medium">
              <m>d^*</m>
            </cell>
            <cell halign="left">
              <m>=f</m>
            </cell>
          </row>
        </tabular>
      </p>
      

    </introduction>

    <task>
      <statement>
        <p>
          Let <m>y_i^*=-c^*_?</m> if <m>c_?^*</m> is the coefficient for <m>t_i</m>
          in the optimal tableau, and let <m>y^*_i=0</m> otherwise.  Similarly let 
          <m>s_j^*=-c^*_?</m> if <m>c_?^*</m> is the coefficient for <m>x_j</m>
          in the optimal tableau, and let <m>s^*_j=0</m> otherwise.
        </p>
        <p>
          Recall that the optimal tableau represents a reformulation of the original
          problem where  <m>f=c_1x_1+c_2x_2+c_3x_3+c_4x_4</m> is instead rewritten as
          <m>f=c_1^*t_3+c_2^*x_3+c_3^*x_1+c_4^*t_2-d^*</m>.

        </p>
        <p>
          Why must <me>\displaystyle \sum_{j=1}^4 c_jx_j =  \sum_{i=1}^4y_i^*(-t_i) + \sum_{j=1}^4 s_i^*(-x_i)-d^*?</me>
        </p>
      </statement>
    </task>
    <task>
      <statement>
        <p>
          Use the fact that <m>t_i = b_i-\left(\displaystyle \sum_{j=1}^4 a_{ij}x_j\right)</m>
          to rewrite the above equality without <m>t_i</m>'s.  Regroup the right hand side so we have the form:
          <me>\displaystyle \sum_{j=1}^4 c_jx_j = (\text{linear function in terms of }x_j\text{'s})+(\text{constant}).</me>
        </p>
      </statement>
    </task>
    <task>
      <statement>
        <p>
          Recall that the above equality we established is an equality
          <em>as functions of the <m>x_j</m>'s </em>.  What must be the constant portion
          of the right hand side be equal to?  What must the linear function in terms of <m>x_j</m>'s 
          on the right hand side be equal to?
        </p>
      </statement>
    </task>
    <task>
      <statement>
        <p>
          Prove that <m>g(\y^*)=\displaystyle \sum_{i=1}^3 y_i^*b_i=-d^*.</m>
        </p>
      </statement>
    </task>
    <task>
      <statement>
        <p>
          We now need to show that these <m>y_i^*</m>'s we found is a feasible
          solution to the dual problem.  Why do we have that <m>c_j = \displaystyle \sum_{i=1}^4 y_i^*a_{ij}-s_j^*</m>?
        </p>
      </statement>
    </task>
    <task>
      <statement>
        <p>
          Why is each <m>y_i^*, s_j^*\geq 0</m>?  Why does this show that <m>\displaystyle \sum_{i=1}^4 y_i^*a_{ij} \geq c_j</m>?
          This shows that <m>s_j</m>'s are non-negative slack variables for the <m>y_i</m> and
          that the <m>y_i^*</m>'s are a feasible solution.
        </p>
      </statement>
    </task>
    <task>
      <statement>
        <p>
          Show by Weak Duality <xref ref="prop-weakduality"/> that the <m>y_i^*</m>'s
          are an optimal dual solution.
        </p>
      </statement>
    </task>
    
  </activity>

  <activity>
    <statement>
      <p>
        Adopt the arguments of <xref ref="activity-sampleSD"/> to prove 
        the Strong Duality Theorem <xref ref="thm-strongduality"/> for a general
        primal-dual optimization problem
        <tabular halign="center">
          <row>
            <cell halign="left">
            </cell>
            <cell bottom="medium">
              <m>x_1</m>
            </cell>
            <cell bottom="medium">
              <m>x_2</m>
            </cell>
            <cell bottom="medium">
              <m>\cdots</m>
            </cell>
            <cell bottom="medium">
              <m>x_m</m>
            </cell>
            <cell bottom="medium">
              <m>-1</m>
            </cell>
            <cell halign="left">
            </cell>
          </row>
          <row>
            <cell halign="left" right="medium">
            </cell>
            <cell>
              <m>a_{11}</m>
            </cell>
            <cell>
              <m>a_{12}</m>
            </cell>
            <cell>
              <m>\cdots</m>
            </cell>
            <cell right="medium">
              <m>a_{1m}</m>
            </cell>
            <cell right="medium">
              <m>b_1</m>
            </cell>
            <cell halign="left">
              <m>=-t_1</m>
            </cell>
          </row>
          <row>
            <cell halign="left" right="medium">
            </cell>
            <cell>
              <m>a_{21}</m>
            </cell>
            <cell>
              <m>a_{22}</m>
            </cell>
            <cell>
              <m>\cdots</m>
            </cell>
            <cell right="medium">
              <m>a_{2m}</m>
            </cell>
            <cell right="medium">
              <m>b_2</m>
            </cell>
            <cell halign="left">
              <m>=-t_2</m>
            </cell>
          </row>
          <row>
            <cell halign="left" right="medium">
            </cell>
            <cell>
              <m>\vdots</m>
            </cell>
            <cell>
              <m>\vdots</m>
            </cell>
            <cell>
              <m>\ddots</m>
            </cell>
            <cell right="medium">
              <m>\vdots</m>
            </cell>
            <cell right="medium">
              <m>\vdots</m>
            </cell>
            <cell halign="left">
              <m>\vdots</m>
            </cell>
          </row>
          
          <row>
            <cell halign="left" right="medium">
            </cell>
            <cell bottom="medium">
              <m>a_{n1}</m>
            </cell>
            <cell bottom="medium">
              <m>a_{n2}</m>
            </cell>
            <cell bottom="medium">
              <m>\cdots</m>
            </cell>
            <cell right="medium" bottom="medium">
              <m>a_{nm}</m>
            </cell>
            <cell right="medium" bottom="medium">
              <m>b_n</m>
            </cell>
            <cell halign="left">
              <m>=-t_n</m>
            </cell>
          </row>
          <row>
            <cell halign="left" right="medium">
            </cell>
            <cell bottom="medium">
              <m>c_1</m>
            </cell>
            <cell bottom="medium">
              <m>c_2</m>
            </cell>
            <cell bottom="medium">
              <m>\cdots</m>
            </cell>
            <cell right="medium" bottom="medium">
              <m>c_m</m>
            </cell>
            <cell right="medium" bottom="medium">
              <m>0</m>
            </cell>
            <cell halign="left">
            </cell>
          </row>
        </tabular>
        which also achieves optimality for some general tableau.
      </p>
      <p>
        Use the facts that <me>\displaystyle \sum_{j=1}^m c_jx_j =  \sum_{i=1}^ny_i^*(-t_i) + \sum_{j=1}^m s_i^*(-x_i)-d^*,</me>
        that <m>t_i = b_i-\left(\displaystyle \sum_{j=1}^n a_{ij}x_j\right)</m>, and  by construction
        each <m>y_i^*, s_j^*\geq0</m>.
      </p>
    </statement>
  </activity>

  <p>
    An alternative approach to proving this theorem is provided in <xref ref="sec-altduality"/>.
  </p>


  

  <activity>
    <title>Complementary Slackness</title>
    <introduction>
      <p>
        We assume the primal problem is canonical.
      </p>
    </introduction>
    <task>
      <statement>
        <p>
          Prove that <m>g-f = \vs^\top\x + \y^\top\vt </m>.
        </p>
      </statement>
    </task>

    <task>
      <statement>
        <p>
          Suppose <m>\x</m> is a  feasible extreme point, and <m>\y, \vs</m> are the corresponding coefficients for the normal vectors.   If <m>x_j\neq 0</m>, what does that
          say about <m>s_j</m>?
        </p>
        <hint>
          <statement>
          <p>
            <m>s_j</m> is the coefficient of the normal vector for the plane <m>-x_j=0</m>.  If
            the feasible solution does not lie on <m>-x_j=0</m>, what can we say about <m>s_j</m>?
          </p>
          </statement>
        </hint>
        <p>
          What about <m>s_j\neq 0</m>?, <m>y_i\neq0</m>? <m>t_i\neq0</m>?
        </p>
      </statement>
    </task>

    <task>
      <statement>
        <p>
          Give an example of a linear optimization primal-dual problem, and feasible solutions 
          <m>\x, \y</m> with slack variables <m>\vt, \vs</m> where <m> \vs^\top\x + \y^\top\vt &gt; 0</m>.
        </p>
        
      </statement>
    </task>

    <task>
      <statement>
        <p>
          If <m>\x^*, \y^*</m> are feasible optimal solutions with slack variables <m>\vt^*, \vs^*</m>, what must be true about <m>(\vs^*)^\top\x^* + (\y^*)^\top\vt^*</m>?
        </p>
      
      </statement>
      
    </task>
    
  </activity>

  <definition xml:id="def-complementaryslackness">
    <idx>complementary slackness</idx>
    <statement>
      <p>
        Feasible variables <m>\x, \y</m> with slack variables <m> \vs, \vt </m> are said to exhibit <term>complementary slackness</term> if 
          <m>\vs^\top\x=0, \y^\top\vt=0</m>.
          
      </p>
    </statement>
  </definition>

  
  
  


  
  



  

</section>